Isabelle/StateTransition.thy
@@ -235,6 +235,10 @@ lemma (in Protocol) state_differences_have_immediately_next_messages:
   using strict_subset_of_state_have_immediately_next_messages
   by (simp add: psubsetI)
 
+(* ###################################################### *)
+(* Union of states is state *)
+(* ###################################################### *)
+
 lemma (in Protocol) union_of_two_states_is_state :
   "\<forall> \<sigma>1 \<in> \<Sigma>. \<forall> \<sigma>2 \<in> \<Sigma>. (\<sigma>1 \<union> \<sigma>2) \<in> \<Sigma>"
   apply (rule, rule)
@@ -337,37 +341,115 @@ proof -
 qed
 
 
-lemma (in Protocol) non_empty_state_is_reached_by_receiving_single_message :
-  "\<forall> \<sigma> \<in> \<Sigma>. \<sigma> \<noteq> \<emptyset> \<longrightarrow> (\<exists> \<sigma>' m. \<sigma>' \<in> \<Sigma> \<and> m \<in> \<sigma> \<and> m \<notin> \<sigma>' \<and> \<sigma> = \<sigma>' \<union> {m})"
-  sorry
+(* ###################################################### *)
+(* MessagePath *)
+(* ###################################################### *)
 
-lemma (in Protocol) non_empty_state_is_reached_by_receiving_immediately_next_message :
-  "\<forall> \<sigma> \<in> \<Sigma>. \<sigma> \<noteq> \<emptyset> \<longrightarrow> (\<exists> \<sigma>' m. \<sigma>' \<in> \<Sigma> \<and> m \<in> \<sigma> \<and> immediately_next_message(\<sigma>', m) \<and> \<sigma> = \<sigma>' \<union> {m})"
-  using state_differences_have_immediately_next_messages 
-        state_transition_only_made_by_immediately_next_message 
-        non_empty_state_is_reached_by_receiving_single_message
-  by (metis message_in_state_is_valid)
+inductive (in Protocol) MessagePath :: "state \<Rightarrow> state \<Rightarrow> message list \<Rightarrow> bool" where
+  P_nil: "MessagePath \<sigma> \<sigma> []"
+| P_cons: "\<lbrakk> immediately_next_message (\<sigma>, m); \<sigma> \<union> {m} \<in> \<Sigma>; MessagePath (\<sigma> \<union> {m}) \<sigma>' list \<rbrakk> \<Longrightarrow> MessagePath \<sigma> \<sigma>' (m # list)"
 
-lemma (in Protocol) intermediate_state_before_receiving_single_message :
-  "\<forall> \<sigma> \<sigma>'. {\<sigma>, \<sigma>'} \<subseteq> \<Sigma> \<and> \<sigma> \<subset> \<sigma>' \<and> \<sigma>' \<noteq> \<emptyset> 
-  \<longrightarrow> (\<exists> \<sigma>'' m. \<sigma>'' \<in> \<Sigma> \<and> m \<in> \<sigma>' \<and> immediately_next_message(\<sigma>'', m) \<and> \<sigma>' = \<sigma>'' \<union> {m} \<and> \<sigma> \<subseteq> \<sigma>'')"
-  apply (rule, rule, rule)
-proof -
-  fix \<sigma> \<sigma>'
-  assume "{\<sigma>, \<sigma>'} \<subseteq> \<Sigma> \<and> \<sigma> \<subset> \<sigma>' \<and> \<sigma>' \<noteq> \<emptyset>"
-  then have "\<exists> \<sigma>'' m. \<sigma>'' \<in> \<Sigma> \<and> m \<in> \<sigma>' \<and> immediately_next_message(\<sigma>'', m) \<and> \<sigma>' = \<sigma>'' \<union> {m}"
-    using non_empty_state_is_reached_by_receiving_immediately_next_message
-    by simp    
-  then obtain \<sigma>'' m where "\<sigma>'' \<in> \<Sigma> \<and> m \<in> \<sigma>' \<and> immediately_next_message(\<sigma>'', m) \<and> \<sigma>' = \<sigma>'' \<union> {m}"
+lemma (in Protocol) exist_message_path_nonnil:
+  assumes "\<sigma>' \<in> futures \<sigma>"
+  and "\<sigma> \<in> \<Sigma>" "\<sigma>' \<in> \<Sigma>" "\<sigma> \<noteq> \<sigma>'"
+  obtains message_list where "MessagePath \<sigma> \<sigma>' message_list"
+proof-
+  have "finite \<sigma> \<and> finite \<sigma>'"
+    using assms(1)
+    unfolding futures_def \<Sigma>t_def
+    using rev_finite_subset state_is_finite by fastforce
+  obtain d where "d = \<sigma>' - \<sigma>"
     by auto
-  then have "\<sigma> \<subset> \<sigma>' \<and> \<sigma>' \<noteq> \<emptyset> \<and> \<sigma>' = \<sigma>'' \<union> {m} \<and> m \<in> \<sigma>' \<and> m \<notin> \<sigma>''"
-    apply (simp add: immediately_next_message_def)
-    using \<open>{\<sigma>, \<sigma>'} \<subseteq> \<Sigma> \<and> \<sigma> \<subset> \<sigma>' \<and> \<sigma>' \<noteq> \<emptyset>\<close> by auto    
-  then have "\<sigma> \<subseteq> \<sigma>''"    
-    sorry
-  then show "\<exists>\<sigma>'' m. \<sigma>'' \<in> \<Sigma> \<and> m \<in> \<sigma>' \<and> immediately_next_message (\<sigma>'', m) \<and> \<sigma>' = \<sigma>'' \<union> {m} \<and> \<sigma> \<subseteq> \<sigma>''"
-    using \<open>\<sigma>'' \<in> \<Sigma> \<and> m \<in> \<sigma>' \<and> immediately_next_message (\<sigma>'', m) \<and> \<sigma>' = \<sigma>'' \<union> {m}\<close> by blast
+  have "finite d"
+    by (simp add: \<open>d = \<sigma>' - \<sigma>\<close> \<open>finite \<sigma> \<and> finite \<sigma>'\<close>)
+
+  assume "\<And>message_list. MessagePath \<sigma> \<sigma>' message_list \<Longrightarrow> thesis"
+
+  {
+    fix n
+    have "\<lbrakk> n = card (\<sigma>' - \<sigma>); finite \<sigma>; finite \<sigma>'; \<sigma> \<noteq> \<sigma>'; \<sigma> \<in> \<Sigma>; \<sigma>' \<in> \<Sigma>; \<sigma> \<subseteq> \<sigma>' \<rbrakk> \<Longrightarrow> \<exists>message_list. MessagePath \<sigma> \<sigma>' message_list \<and> length message_list = n"
+      apply (induct n arbitrary: \<sigma> \<sigma>' d)
+      apply (simp)
+    proof simp
+      fix n and \<sigma> :: state and \<sigma>'
+      assume "\<And>\<sigma> \<sigma>'.
+           n = card (\<sigma>' - \<sigma>) \<Longrightarrow>
+           finite \<sigma> \<Longrightarrow>
+           finite \<sigma>' \<Longrightarrow>
+           \<sigma> \<noteq> \<sigma>' \<Longrightarrow>
+           \<sigma> \<in> \<Sigma> \<Longrightarrow> \<sigma>' \<in> \<Sigma> \<Longrightarrow> \<sigma> \<subseteq> \<sigma>' \<Longrightarrow> \<exists>message_list. MessagePath \<sigma> \<sigma>' message_list \<and> length message_list = card (\<sigma>' - \<sigma>)"
+        and "Suc n = card (\<sigma>' - \<sigma>)" "finite \<sigma>" "finite \<sigma>'" "\<sigma> \<noteq> \<sigma>'" "\<sigma> \<in> \<Sigma>" "\<sigma>' \<in> \<Sigma>" "\<sigma> \<subseteq> \<sigma>'"
+
+      obtain m where "immediately_next_message (\<sigma>, m)" "m \<in> \<sigma>' - \<sigma>" 
+        using state_differences_have_immediately_next_messages
+        by (meson \<open>\<sigma> \<noteq> \<sigma>'\<close> \<open>\<sigma> \<subseteq> \<sigma>'\<close> \<open>\<sigma>' \<in> \<Sigma>\<close> psubsetI strict_subset_of_state_have_immediately_next_messages)
+      have cardn: "card (\<sigma>' - (\<sigma> \<union> {m})) = n"
+        using \<open>Suc n = card (\<sigma>' - \<sigma>)\<close> \<open>finite \<sigma>'\<close> \<open>m \<in> \<sigma>' - \<sigma>\<close> by auto
+      have "finite (\<sigma> \<union> {m})"
+        by (simp add: \<open>finite \<sigma>\<close>)
+      have "\<sigma> \<union> {m} \<in> \<Sigma>"
+        using \<open>\<sigma> \<in> \<Sigma>\<close> \<open>\<sigma>' \<in> \<Sigma>\<close> \<open>immediately_next_message (\<sigma>, m)\<close> \<open>m \<in> \<sigma>' - \<sigma>\<close> message_in_state_is_valid state_transition_by_immediately_next_message by fastforce
+      have "\<sigma> \<union> {m} \<subseteq> \<sigma>'"
+        using \<open>\<sigma> \<subseteq> \<sigma>'\<close> \<open>m \<in> \<sigma>' - \<sigma>\<close> by auto
+      have "m \<notin> \<sigma>"
+        using \<open>m \<in> \<sigma>' - \<sigma>\<close> by auto
+
+      obtain message_list where "MessagePath \<sigma> \<sigma>' message_list \<and> length message_list = Suc n"
+      proof (cases "\<sigma> \<union> {m} = \<sigma>'")
+        case True
+        assume "\<And>message_list. MessagePath \<sigma> \<sigma>' message_list \<and> length message_list = Suc n \<Longrightarrow> thesis"
+        have "\<sigma>' - (\<sigma> \<union> {m}) = \<emptyset>"
+          using True by auto
+        hence "card (\<sigma>' - (\<sigma> \<union> {m})) = 0"
+          by (metis card_empty)
+        hence "n = 0"
+          using cardn by simp
+        have "MessagePath \<sigma> \<sigma>' [m]"
+          using P_cons True \<open>immediately_next_message (\<sigma>, m)\<close> 
+          using P_nil \<open>\<sigma> \<union> {m} \<in> \<Sigma>\<close> by auto
+        have "length [m] = Suc 0"
+          by simp
+        show ?thesis
+          using \<open>MessagePath \<sigma> \<sigma>' [m]\<close> \<open>length [m] = Suc 0\<close> \<open>n = 0\<close> that by blast
+      next
+        case False
+        assume "\<And>message_list. MessagePath \<sigma> \<sigma>' message_list \<and> length message_list = Suc n \<Longrightarrow> thesis"
+        obtain prev_list where "MessagePath (\<sigma> \<union> {m}) \<sigma>' prev_list \<and> length prev_list = card (\<sigma>' - (\<sigma> \<union> {m}))"
+          using False \<open>\<And>\<sigma>' \<sigma>. \<lbrakk>n = card (\<sigma>' - \<sigma>); finite \<sigma>; finite \<sigma>'; \<sigma> \<noteq> \<sigma>'; \<sigma> \<in> \<Sigma>; \<sigma>' \<in> \<Sigma>; \<sigma> \<subseteq> \<sigma>'\<rbrakk> \<Longrightarrow> \<exists>message_list. MessagePath \<sigma> \<sigma>' message_list \<and> length message_list = card (\<sigma>' - \<sigma>)\<close> \<open>\<sigma> \<union> {m} \<in> \<Sigma>\<close> \<open>\<sigma> \<union> {m} \<subseteq> \<sigma>'\<close> \<open>\<sigma>' \<in> \<Sigma>\<close> \<open>finite (\<sigma> \<union> {m})\<close> \<open>finite \<sigma>'\<close> cardn by blast
+        have "MessagePath \<sigma> \<sigma>' (m # prev_list)"
+          using P_cons \<open>MessagePath (\<sigma> \<union> {m}) \<sigma>' prev_list \<and> length prev_list = card (\<sigma>' - (\<sigma> \<union> {m}))\<close> \<open>immediately_next_message (\<sigma>, m)\<close>
+                \<open>\<sigma> \<union> {m} \<in> \<Sigma>\<close> by blast 
+        then show ?thesis
+          using \<open>MessagePath (\<sigma> \<union> {m}) \<sigma>' prev_list \<and> length prev_list = card (\<sigma>' - (\<sigma> \<union> {m}))\<close> cardn length_Suc_conv that by blast
+      qed
+
+      then show "\<exists>message_list. MessagePath \<sigma> \<sigma>' message_list \<and> length message_list = card (\<sigma>' - \<sigma>)"
+        using \<open>Suc n = card (\<sigma>' - \<sigma>)\<close> by auto
+    qed
+  }
+
+  then show ?thesis
+    using Params.state_is_finite assms(1) assms(2) assms(3) assms(4) futures_def that by fastforce
 qed
+
+lemma (in Protocol) coherent_nonnil_message_path:
+  assumes "MessagePath \<sigma> \<sigma>' message_list" "length message_list \<noteq> 0"
+  obtains m ms where "message_list = m # ms" "MessagePath (\<sigma> \<union> {m}) \<sigma>' ms" "immediately_next_message (\<sigma>,m)" "\<sigma> \<union> {m} \<in> \<Sigma>"
+  using assms
+  apply (cases rule: MessagePath.cases)
+   apply simp
+  by blast
+
+lemma (in Protocol) coherent_nil_message_path: "MessagePath \<sigma> \<sigma>' [] \<Longrightarrow> \<sigma> = \<sigma>'"
+  using MessagePath.cases by blast
+
+lemma (in Protocol) coherent_message_path_inclusive: "MessagePath \<sigma> \<sigma>' ms \<Longrightarrow> \<sigma> \<subseteq> \<sigma>'"
+  by (induct rule: MessagePath.induct, auto)
+
+lemma (in Protocol) exist_message_path:
+  assumes "\<sigma>' \<in> futures \<sigma>" "\<sigma> \<in> \<Sigma>" "\<sigma>' \<in> \<Sigma>"
+  obtains message_list where "MessagePath \<sigma> \<sigma>' message_list"
+  using P_nil Protocol.exist_message_path_nonnil Protocol_axioms assms(1) assms(2) assms(3) by blast
 
 
 (* ###################################################### *)
@@ -474,12 +556,4 @@ proof -
     (* by (smt Diff_iff \<Sigma>t_is_subset_of_\<Sigma> is_singleton_the_elem singletonD subsetCE) *)
 oops
     
-
-lemma (in Protocol) road_to_future_state :
-  "\<forall> \<sigma> \<sigma>'. \<sigma> \<in> \<Sigma> \<and> \<sigma>' \<in> \<Sigma> \<and> is_future_state(\<sigma>, \<sigma>')
-  \<longrightarrow> n = card (\<sigma>' - \<sigma>)  
-  \<longrightarrow> (\<exists> f. f 0 = \<sigma> \<and> f n = \<sigma>' \<and> (\<forall> i. 0 \<le> i \<and> i \<le> n - 1 \<longrightarrow> f i \<in> \<Sigma> \<and> (\<exists> m \<in> M. f i \<union> {m} = f (Suc i))))" 
-  apply (rule, rule, rule, rule) 
-  oops
-
 end
